Cleanup naming conventions

theories/Context.v
@@ -2,6 +2,7 @@ Require Import Blech.Spec.
 Require Blech.Map.
 Require Import Blech.SpecNotations.
 
+Require Import Coq.Unicode.Utf8.
 Require Import Coq.Classes.SetoidClass.
 Require Coq.Lists.List.
 Require Import Coq.Logic.FunctionalExtensionality.
@@ -9,25 +10,33 @@ Require Import Coq.Logic.PropExtensionality.
 
 Require Import FunInd.
 
+Import Map.MapNotations.
 Import List.ListNotations.
 Import IfNotations.
 
-Function typecheck (Γ: linear) (E: context): option (linear * type) :=
+Implicit Type Δ: linear.
+Implicit Type E: context.
+Implicit Type t: type.
+Implicit Type N: normal.
+Implicit Types X Y: cvar.
+Implicit Type σ: store.
+
+Function typecheck Δ E: option (linear * type) :=
   match E with
-  | E_var x =>
-      if Map.find x Γ is Some t
+  | E_var X =>
+      if Map.find X Δ is Some t
       then
-          Some (Map.one x t, t)
+          Some (Map.one X t, t)
       else
         None
-  | E_lam x t1 E =>
-      if typecheck (Map.add x t1 Γ) E is Some (Γ', t2)
+  | E_lam X t1 E =>
+      if typecheck (Map.add X t1 Δ) E is Some (Δ', t2)
       then
-        if Map.find x Γ' is Some t1'
+        if Map.find X Δ' is Some t1'
         then
           if eq_type t1 t1'
           then
-              Some (Map.minus x Γ', t1 * t2)
+              Some (Δ' \ X, t1 * t2)
           else
             None
         else
@@ -35,13 +44,13 @@ Function typecheck (Γ: linear) (E: context): option (linear * type) :=
       else
         None
   | E_app E E' =>
-      if typecheck Γ E is Some (Γ', t1 * t2)
+      if typecheck Δ E is Some (Δ', t1 * t2)
       then
-        if typecheck Γ E' is Some (Δ, t1')
+        if typecheck Δ E' is Some (Δ, t1')
         then
           if eq_type t1 t1'
           then
-            Some (Map.merge Γ' Δ, t2)
+            Some (Δ' ∪ Δ, t2)
           else
             None
         else
@@ -51,41 +60,41 @@ Function typecheck (Γ: linear) (E: context): option (linear * type) :=
 
   | E_tt => Some (Map.empty, t_unit)
   | E_step E E' =>
-      if typecheck Γ E is Some (Γ', t_unit)
+      if typecheck Δ E is Some (Δ', t_unit)
       then
-        if typecheck Γ E' is Some (Δ, t)
+        if typecheck Δ E' is Some (Δ, t)
         then
-          Some (Map.merge Γ' Δ, t)
+          Some (Δ' ∪ Δ, t)
         else
           None
       else
         None
 
   | E_fanout E E' =>
-      if typecheck Γ E is Some (Γ', t1)
+      if typecheck Δ E is Some (Δ', t1)
       then
-        if typecheck Γ E' is Some (Δ, t2)
+        if typecheck Δ E' is Some (Δ, t2)
         then
-          Some (Map.merge Γ' Δ, t_prod t1 t2)
+          Some (Δ' ∪ Δ, t_prod t1 t2)
         else
           None
       else
         None
 
-  | E_let x y E E' =>
-      if typecheck Γ E is Some (Γ', t1 * t2)
+  | E_let X Y E E' =>
+      if typecheck Δ E is Some (Δ', t1 * t2)
       then
-        if typecheck (Map.add x t1 (Map.add y t2 Γ)) E' is Some (Δ, t3)
+        if typecheck (Map.add X t1 (Map.add Y t2 Δ)) E' is Some (Δ, t3)
         then
-          if Map.find x (Map.minus y Δ) is Some t1'
+          if Map.find X (Δ \ Y) is Some t1'
           then
             if eq_type t1 t1'
             then
-              if Map.find y Δ is Some t2'
+              if Map.find Y Δ is Some t2'
               then
                 if eq_type t2 t2'
                 then
-                  Some (Map.merge Γ' (Map.minus x (Map.minus y Δ)), t3)
+                  Some (Δ' ∪ ((Δ \ Y) \ X), t3)
                 else
                   None
               else
@@ -102,10 +111,10 @@ Function typecheck (Γ: linear) (E: context): option (linear * type) :=
     %list.
 
 Theorem typecheck_sound:
-  forall Γ {E Δ t}, typecheck Γ E = Some (Δ, t) -> Δ ⊢ E ? t.
+  ∀ Δ {E Δ' t}, typecheck Δ E = Some (Δ', t) → Δ' ⊢ E ? t.
 Proof using.
-  intros Γ E.
-  functional induction (typecheck Γ E).
+  intros Δ E.
+  functional induction (typecheck Δ E).
   all: cbn.
   all: intros ? ? p.
   all: inversion p.
@@ -113,7 +122,7 @@ Proof using.
   all: econstructor.
   all: eauto.
   - apply IHo.
-    rewrite (Map.add_minus x t1 Γ').
+    rewrite (Map.add_minus X t1 Δ').
     2: auto.
     auto.
   - rewrite Map.add_minus.
@@ -124,7 +133,7 @@ Qed.
 
 Notation "'do' x <- e0 ; e1" := (List.flat_map (fun x => e1) e0) (x pattern, at level 200, left associativity).
 
-Fixpoint app {A B} (f: list (A -> B)) x: list _ :=
+Fixpoint app {A B} (f: list (A → B)) x: list _ :=
   if f is cons H T
   then
     List.app (List.map H x) (app T x)
@@ -133,24 +142,24 @@ Fixpoint app {A B} (f: list (A -> B)) x: list _ :=
 
 Infix "<*>" := app (at level 30).
 
-Fixpoint generate (t: type): list normal :=
+Fixpoint generate t :=
   match t with
   | t_unit => [N_tt]
   | A * B => [N_fanout] <*> generate A <*> generate B
   end%list.
 
-Fixpoint search (σ: Map.map normal) E: list span :=
+Fixpoint search σ E: list span :=
   match E with
-  | E_var x => if Map.find x σ is Some N then [Map.one x N |- N] else []
+  | E_var X => if Map.find X σ is Some N then [Map.one X N |- N] else []
 
-  | E_lam x t E =>
+  | E_lam X t E =>
       do N0 <- generate t ;
-      do (σ' |- N1) <- search (Map.add x N0 σ) E ;
-      if Map.find x σ' is Some N0'
+      do (σ' |- N1) <- search (Map.add X N0 σ) E ;
+      if Map.find X σ' is Some N0'
       then
         if eq_normal N0 N0'
         then
-          [Map.minus x σ' |- N_fanout N0 N1]
+          [Map.minus X σ' |- N_fanout N0 N1]
         else
           []
       else
@@ -163,7 +172,7 @@ Fixpoint search (σ: Map.map normal) E: list span :=
       then
         if eq_normal N0 N0'
         then
-          [Map.merge σ1 σ2 |- N1]
+          [(σ1 ∪ σ2) |- N1]
         else
           []
       else
@@ -175,26 +184,26 @@ Fixpoint search (σ: Map.map normal) E: list span :=
       do (σ1 |- N) <- search σ E ;
       if N is N_tt
       then
-        [fun '(σ2 |- N') => Map.merge σ1 σ2 |- N'] <*> search σ E'
+        [fun '(σ2 |- N') => (σ1 ∪ σ2) |- N'] <*> search σ E'
       else
         []
 
   | E_fanout E E' =>
-      [fun '(σ1 |- N) '(σ2 |- N') => Map.merge σ1 σ2 |- N_fanout N N'] <*> search σ E <*> search σ E'
+      [fun '(σ1 |- N) '(σ2 |- N') => (σ1 ∪ σ2) |- N_fanout N N'] <*> search σ E <*> search σ E'
 
-  | E_let x y E E' =>
+  | E_let X Y E E' =>
       do (σ1 |- N) <- search σ E ;
       do (a, b) <- (if N is N_fanout a b then [(a, b)] else []) ;
-      do (σ2 |- N') <- search (Map.add x a (Map.add y b σ)) E' ;
-      if Map.find x (Map.minus y σ2)is Some a'
+      do (σ2 |- N') <- search (Map.add X a (Map.add Y b σ)) E' ;
+      if Map.find X (Map.minus Y σ2)is Some a'
       then
         if eq_normal a a'
         then
-          if Map.find y σ2 is Some b'
+          if Map.find Y σ2 is Some b'
           then
             if eq_normal b b'
             then
-              [Map.merge σ1 (Map.minus x (Map.minus y σ2)) |- N']
+              [σ1 ∪ ((σ2 \ Y) \ X) |- N']
             else
               []
           else
@@ -205,16 +214,15 @@ Fixpoint search (σ: Map.map normal) E: list span :=
         []
   end%list.
 
-Lemma sound_pure {E S N}: sat E S N -> sound E ([S |- N]%list).
+Lemma sound_pure:
+  ∀ {E S N}, sat E S N → sound E ([S |- N]%list).
 Proof.
-  intro.
-  constructor.
-  1: constructor.
+  repeat constructor.
   auto.
 Defined.
 
 Lemma sound_mon {E p p'}:
-  sound E p -> sound E p' ->
+  sound E p → sound E p' →
   sound E ((p ++ p')%list).
 Proof.
   intros.
@@ -227,7 +235,7 @@ Proof.
 Defined.
 
 Lemma sound_fst {E p p'}:
-  sound E ((p ++ p')%list) ->
+  sound E ((p ++ p')%list) →
   sound E p.
 Proof.
   intros.
@@ -242,7 +250,7 @@ Proof.
 Defined.
 
 Lemma sound_snd {E p p'}:
-  sound E ((p ++ p')%list) ->
+  sound E ((p ++ p')%list) →
   sound E p'.
 Proof.
   intros.
@@ -256,7 +264,7 @@ Proof.
 Defined.
 
 Lemma sound_split {E p p'}:
-  sound E ((p ++ p')%list) -> sound E p * sound E p'.
+  sound E ((p ++ p')%list) → sound E p * sound E p'.
 Proof.
   intros.
   refine (sound_fst _, sound_snd _).
@@ -264,7 +272,7 @@ Proof.
 Defined.
 
 Theorem search_sound:
-  forall σ E, sound E (search σ E).
+  ∀ σ E, sound E (search σ E).
 Proof using.
   intros σ E.
   generalize dependent σ.
@@ -383,7 +391,7 @@ Proof using.
 Qed.
 
 Theorem search_sound_sat:
-  forall σ E N, List.In (σ |- N) (search σ E) -> sat E σ N.
+  ∀ σ E N, List.In (σ |- N) (search σ E) → sat E σ N.
 Proof using.
   intros σ E.
   induction (search_sound σ E).
@@ -397,27 +405,27 @@ Proof using.
   auto.
 Defined.
 
-(* FIXME make a monad ? *)
+(* FIXME put elsewhere/make a monad? *)
 Section Heap.
   Context {A: Type}.
 
-  Definition hprop := A -> store -> Prop.
+  Definition hprop := A → store → Prop.
 
   Inductive hempty: hprop :=
   | hempty_intro {a}: hempty a Map.empty.
 
   Inductive hpure P: hprop :=
-  | hpure_intro {a}: P -> hpure P a Map.empty.
+  | hpure_intro {a}: P → hpure P a Map.empty.
 
   Inductive hsingle X N: hprop :=
   | hsingle_intro {a}: hsingle X N a (Map.one X N).
 
   Inductive hstar (H H': hprop): hprop :=
   | hstar_intro {a h1 h2}:
-    H a h1 -> H' a h2 -> Map.disjoint h1 h2 ->
+    H a h1 → H' a h2 → Map.disjoint h1 h2 →
     hstar H H' a (Map.merge h1 h2).
-  Inductive hexists {A} (J: A -> hprop): hprop :=
-  | hexists_intro {x a h}: J x a h -> hexists J a h.
+  Inductive hexists {A} (J: A → hprop): hprop :=
+  | hexists_intro {x a h}: J x a h → hexists J a h.
 End Heap.
 
 Arguments hprop: clear implicits.
@@ -435,7 +443,7 @@ Notation "'\exists' x1 .. xn , H" :=
 Definition ig {A} (P: hprop unit): hprop A := fun _ => P tt.
 
 Theorem hstar_assoc:
-  forall {V} {A B C: hprop V},
+  ∀ {V} {A B C: hprop V},
     (A \* B) \* C = A \* (B \* C).
 Proof using.
   intros ? A B C.
@@ -521,25 +529,25 @@ Qed.
 (* Satisfaction defines a sort of nondeterministic Hoare logic *)
 
 (* based on https://softwarefoundations.cis.upenn.edu/slf-current/Hprop.html *)
-Inductive eval: context -> store -> normal -> store -> Prop :=
-| eval_sat {E σ σ' N}: sat E σ' N -> eval E σ N (Map.merge σ σ').
+Inductive eval: context → store → normal → store → Prop :=
+| eval_sat {E σ σ' N}: sat E σ' N → eval E σ N (Map.merge σ σ').
 
 Definition hoare E (H: hprop unit) (Q: hprop normal): Prop :=
-  forall s,
-    H tt s ->
+  ∀ s,
+    H tt s →
     exists s' N, eval E s N s' /\ Q N s'.
 
 Definition triple E H (Q: hprop normal) : Prop :=
-  forall H', hoare E (H \* H') (Q \* ig H').
+  ∀ H', hoare E (H \* H') (Q \* ig H').
 
 Definition oftype t := { E | Map.empty ⊢ E ? t }.
 
 Definition equiv {t}: Relation_Definitions.relation (oftype t) :=
-  fun E E' =>
-    forall N,
-      sat (proj1_sig E) Map.empty N <-> sat (proj1_sig E') Map.empty N.
+  fun a b =>
+    ∀ N,
+      sat (proj1_sig a) Map.empty N ↔ sat (proj1_sig b) Map.empty N.
 
-Instance equiv_Reflexive A: Reflexive (@equiv A).
+Instance equiv_Reflexive t: Reflexive (@equiv t).
 Proof using.
   unfold equiv.
   unfold Reflexive.
@@ -547,7 +555,7 @@ Proof using.
   reflexivity.
 Qed.
 
-Instance equiv_Symmetric A: Symmetric (@equiv A).
+Instance equiv_Symmetric t: Symmetric (@equiv t).
 Proof using.
   unfold equiv.
   unfold Symmetric.
@@ -556,7 +564,7 @@ Proof using.
   auto.
 Qed.
 
-Instance equiv_Transitive A: Transitive (@equiv A).
+Instance equiv_Transitive t: Transitive (@equiv t).
 Proof using.
   unfold equiv.
   unfold Transitive.
@@ -566,19 +574,19 @@ Proof using.
   reflexivity.
 Qed.
 
-Instance equiv_Equivalence A: Equivalence (@equiv A) := {
+Instance equiv_Equivalence t: Equivalence (@equiv t) := {
     Equivalence_Reflexive := _ ;
 }.
 
-Instance oftype_Setoid A: Setoid (oftype A) := {
+Instance oftype_Setoid t: Setoid (oftype t) := {
     equiv := equiv ;
 }.
 
 
 #[program]
 Definition id t: oftype (t * t) :=
-  let x := 0 in
-  E_lam x t (E_var x).
+  let X := 0 in
+  E_lam X t (E_var X).
 
 Next Obligation.
 Proof.
@@ -592,9 +600,9 @@ Admitted.
 
 #[program]
 Definition conv {t t'} (E: oftype (t * t')): oftype (t' * t) :=
-  let x := 0 in
-  let y := 1 in
-  E_let x y E (E_fanout (E_var y) (E_var x)).
+  let X := 0 in
+  let Y := 1 in
+  E_let X Y E (E_fanout (E_var Y) (E_var X)).
 
 Next Obligation.
 Proof.
